First_Order_Clause: Polymorphic Context

thys/First_Order_Clause/IsaFoR_Nonground_Term.thy
@@ -11,8 +11,23 @@ global_interpretation "term": nonground_term where
   term_from_ground = term_of_gterm and term_is_ground = is_ground
   by unfold_locales
 
-global_interpretation "term": smaller_subterms where
-  subterms = args and size = size and is_var = is_Var
-  by unfold_locales (metis in_set_simps(3) supt.intros(1) supt_size term.exhaust_sel term.sel(3))
+fun fun_sym where
+ "fun_sym (Fun f _) = f"
+
+global_interpretation "term": term_interpretation where
+  subterms = args and size = size and is_var = term.is_Var and Fun = "\<lambda>f _. Fun f" and 
+  fun_sym = fun_sym and extra = "\<lambda>_. ()"
+proof unfold_locales
+  fix t t' :: "('f, 'v) term"
+  assume "t' \<in> set (args t)"
+
+  then show "size t' < size t"
+    by (induction t) (auto simp: size_simp1)
+next
+  fix t :: "('f, 'v) term"
+
+  show "\<not> term.is_Var t \<longleftrightarrow> (\<exists>f e ts. t = Fun f ts)"
+    by (metis Term.term.simps(17,4) empty_not_insert term.exhaust_sel)
+qed auto
 
 end
