thys/First_Order_Clause/Polymorphic_Ground_Term.thy
@@ -7,17 +7,15 @@ begin
 datatype ('f, 'tyf) poly_gterm =
   PGFun (fun_sym: 'f) (type_args: "'tyf gterm list") (args: "('f, 'tyf) poly_gterm list")
 
-interpretation poly_gterm: smaller_subterms where
-  subterms = args and size = size and is_var = "\<lambda>_. False"
+interpretation poly_gterm: term_interpretation where
+  Fun = PGFun and fun_sym = fun_sym and subterms = args and extra = type_args and
+  is_var = is_var and size = size
 proof unfold_locales
   fix t t' :: "('f, 'tyf) poly_gterm"
-  assume "t' \<in> set (poly_gterm.args t)" 
+  assume "t' \<in> set (poly_gterm.args t)"
+
   then show "size t' < size t"
     by (induction t arbitrary: t') (auto simp: elem_size_size_list_size less_SucI trans_less_add2)
-qed
-
-interpretation poly_gterm: term_interpretation where
-  Fun = PGFun and fun_sym = fun_sym and subterms = args and extra = type_args and is_var = is_var
-  by unfold_locales (auto intro: poly_gterm.exhaust)
+qed (auto intro: poly_gterm.exhaust)
 
 end
